Use HL conversions for all data types + Pipeline.v refactors

src/Assembly/GF25519.v
@@ -35,8 +35,24 @@ Module GF25519.
     exact t.
   Defined.
 
-  Definition liftFE {T} (F: @interp_type Z FE -> T) :=
-    fun (a b c d e f g h i j: Z) => F (a, b, c, d, e, f, g, h, i, j).
+  Definition flatten {T}: (@interp_type Z FE -> T) -> NAry 10 Z T.
+    intro F; refine (fun (a b c d e f g h i j: Z) =>
+      F (a, b, c, d, e, f, g, h, i, j)).
+  Defined.
+
+  Definition unflatten {T}:
+      (forall a b c d e f g h i j, T (a, b, c, d, e, f, g, h, i, j))
+    -> (forall x: @interp_type Z FE, T x).
+  Proof.
+    intro F; refine (fun (x: @interp_type Z FE) =>
+      let '(a, b, c, d, e, f, g, h, i, j) := x in
+      F a b c d e f g h i j).
+  Defined.
+
+  Ltac intro_vars_for R := revert R;
+    match goal with
+    | [ |- forall x, @?T x ] => apply (@unflatten T); intros
+    end.
 
   Module AddExpr <: Expression.
     Definition bits: nat := bits.
@@ -51,15 +67,8 @@ Module GF25519.
     Definition ge25519_add' (P Q: @interp_type Z FE) :
         { r: @HL.expr Z (@interp_type Z) FE | HL.interp (t := FE) r = ge25519_add_expr P Q }.
     Proof.
-      vm_compute in P, Q; repeat
-        match goal with
-        | [x:?T |- _] =>
-          lazymatch T with
-          | Z => fail
-          | prod _ _ => destruct x
-          | _ => clear x
-          end
-        end.
+      intro_vars_for P.
+      intro_vars_for Q.
 
       eexists.
       cbv beta delta [ge25519_add_expr].
@@ -78,8 +87,80 @@ Module GF25519.
         proj1_sig (ge25519_add' P Q).
 
     Definition hlProg: NAry 20 Z (@HL.expr Z (@interp_type Z) ResultType) :=
-        liftFE (fun p => (liftFE (fun q => ge25519_add p q))).
+        Eval cbv in (flatten (fun p => (flatten (fun q => ge25519_add p q)))).
   End AddExpr.
+
+  Module SubExpr <: Expression.
+    Definition bits: nat := bits.
+    Definition inputs: nat := 20.
+    Definition width: Width bits := width.
+    Definition ResultType := FE.
+    Definition inputBounds := feBound ++ feBound.
+
+    Definition ge25519_sub_expr :=
+        Eval cbv beta delta [fe25519 carry_add mul carry_sub Let_In] in carry_sub.
+
+    Definition ge25519_sub' (P Q: @interp_type Z FE) :
+        { r: @HL.expr Z (@interp_type Z) FE | HL.interp (t := FE) r = ge25519_sub_expr P Q }.
+    Proof.
+      intro_vars_for P.
+      intro_vars_for Q.
+
+      eexists.
+      cbv beta delta [ge25519_sub_expr].
+
+      let R := HL.rhs_of_goal in
+      let X := HL.reify (@interp_type Z) R in
+      transitivity (HL.interp (t := ResultType) X); [reflexivity|].
+
+      cbv iota beta delta [
+            interp_type interp_binop HL.interp
+            Z.land ZEvaluable eadd esub emul eshiftr eand].
+      reflexivity.
+    Defined.
+
+    Definition ge25519_sub (P Q: @interp_type Z ResultType) :=
+        proj1_sig (ge25519_sub' P Q).
+
+    Definition hlProg: NAry 20 Z (@HL.expr Z (@interp_type Z) ResultType) :=
+        Eval cbv in (flatten (fun p => (flatten (fun q => ge25519_sub p q)))).
+  End SubExpr.
+
+  Module MulExpr <: Expression.
+    Definition bits: nat := bits.
+    Definition inputs: nat := 20.
+    Definition width: Width bits := width.
+    Definition ResultType := FE.
+    Definition inputBounds := feBound ++ feBound.
+
+    Definition ge25519_mul_expr :=
+        Eval cbv beta delta [fe25519 carry_add mul carry_sub Let_In] in mul.
+
+    Definition ge25519_mul' (P Q: @interp_type Z FE) :
+        { r: @HL.expr Z (@interp_type Z) FE | HL.interp (t := FE) r = ge25519_mul_expr P Q }.
+    Proof.
+      intro_vars_for P.
+      intro_vars_for Q.
+
+      eexists.
+      cbv beta delta [ge25519_mul_expr].
+
+      let R := HL.rhs_of_goal in
+      let X := HL.reify (@interp_type Z) R in
+      transitivity (HL.interp (t := ResultType) X); [reflexivity|].
+
+      cbv iota beta delta [
+            interp_type interp_binop HL.interp
+            Z.land ZEvaluable eadd esub emul eshiftr eand].
+      reflexivity.
+    Defined.
+
+    Definition ge25519_mul (P Q: @interp_type Z ResultType) :=
+        proj1_sig (ge25519_mul' P Q).
+
+    Definition hlProg: NAry 20 Z (@HL.expr Z (@interp_type Z) ResultType) :=
+        Eval cbv in (flatten (fun p => (flatten (fun q => ge25519_mul p q)))).
+  End MulExpr.
 
   Module OppExpr <: Expression.
     Definition bits: nat := bits.
@@ -95,15 +176,7 @@ Module GF25519.
         { r: @HL.expr Z (@interp_type Z) FE
         | HL.interp (E := @ZEvaluable bits) (t := FE) r = ge25519_opp_expr P }.
     Proof.
-      vm_compute in P; repeat
-        match goal with
-        | [x:?T |- _] =>
-          lazymatch T with
-          | Z => fail
-          | prod _ _ => destruct x
-          | _ => clear x
-          end
-        end.
+      intro_vars_for P.
 
       eexists.
       cbv beta delta [ge25519_opp_expr zero_].
@@ -123,14 +196,16 @@ Module GF25519.
         proj1_sig (ge25519_opp' P).
 
     Definition hlProg: NAry 10 Z (@HL.expr Z (@interp_type Z) ResultType) :=
-        liftFE (fun p => ge25519_opp p).
+        Eval cbv in (flatten (fun p => ge25519_opp p)).
   End OppExpr.
 
   Module Add := Pipeline AddExpr.
+  Module Sub := Pipeline SubExpr.
+  Module Mul := Pipeline MulExpr.
   Module Opp := Pipeline OppExpr.
 End GF25519.
 
 Extraction "GF25519Add" GF25519.Add.
+Extraction "GF25519Sub" GF25519.Sub.
+Extraction "GF25519Mul" GF25519.Mul.
 Extraction "GF25519Opp" GF25519.Opp.
-
-Eval cbv in GF25519.Add.outputBounds.
